Rename Congruences.lean to AutomataCongr.lean and refactor it

AutomataTheory/AutomataCongr.lean
@@ -4,7 +4,7 @@ Released under Apache 2.0 license as described in the file LICENSE.
 Authors: Ching-Tsun Chou
 -/
 
-import AutomataTheory.RegLang
+import AutomataTheory.AutomataDet
 
 /-!
 A congruence is an equivalence relation on finite sequences that is
@@ -13,7 +13,7 @@ For now, we assume only the right congruence condition.  We will
 add the left congruence condition if and when it is needed.
 -/
 
-open Function Set Filter
+open Function Set
 
 section Congruences
 
@@ -23,7 +23,7 @@ class Congruence (A : Type*) extends eq : Setoid (List A) where
 
 variable {A : Type*}
 
-def AutomataCongr (c : Congruence A) : DetAutomaton A where
+def DetAutomaton.ofCongr (c : Congruence A) : DetAutomaton A where
   State := Quotient c.eq
   init := ⟦ [] ⟧
   next := fun s a ↦ Quotient.lift (fun u ↦ ⟦ u ++ [a] ⟧) ( by
@@ -32,42 +32,29 @@ def AutomataCongr (c : Congruence A) : DetAutomaton A where
 
 variable {c : Congruence A}
 
-theorem automata_congr_run (as : ℕ → A) (n : ℕ) :
-    MakeDetRun (AutomataCongr c) as n = ⟦ List.ofFn (fun k : Fin n ↦ as k) ⟧ := by
+theorem automaton_congr_run (as : ℕ → A) (n : ℕ) :
+    MakeDetRun (DetAutomaton.ofCongr c) as n = ⟦ List.ofFn (fun k : Fin n ↦ as k) ⟧ := by
   induction' n with n h_ind
-  · simp [MakeDetRun, AutomataCongr]
+  · simp [MakeDetRun, DetAutomaton.ofCongr]
   simp only [MakeDetRun, h_ind]
-  simp only [AutomataCongr, Quotient.lift_mk, Quotient.eq]
+  simp only [DetAutomaton.ofCongr, Quotient.lift_mk, Quotient.eq]
   suffices h_eq : ((List.ofFn fun k : Fin n ↦ as ↑k) ++ [as n]) = (List.ofFn fun k : Fin (n + 1) ↦ as ↑k) by
     simp [h_eq, c.eq.iseqv.refl]
   exact Eq.symm List.ofFn_succ_last
 
-theorem accepted_lang_congr [Inhabited A] (s : (AutomataCongr c).State) :
-    AcceptedLang (FromDetAutomaton (AutomataCongr c)) {s} = Quotient.mk c.eq ⁻¹' {s} := by
+theorem accepted_lang_congr [Inhabited A] (s : (DetAutomaton.ofCongr c).State) :
+    AcceptedLang (FromDetAutomaton (DetAutomaton.ofCongr c)) {s} = Quotient.mk c.eq ⁻¹' {s} := by
   ext al ; simp [AcceptedLang, FinAccept] ; constructor
   · rintro ⟨n, as, ⟨ss, h_run, rfl⟩, rfl⟩
     have h_ss_n := det_automata_fin_run_unique h_run n (by omega)
-    simp [h_ss_n, automata_congr_run]
+    simp [h_ss_n, automaton_congr_run]
   · rintro ⟨rfl⟩
     let as := fun k ↦ if h : k < al.length then al[k] else default
     use al.length, as
     constructor <;> [skip ; simp [as]]
-    use (MakeDetRun (AutomataCongr c) as)
+    use (MakeDetRun (DetAutomaton.ofCongr c) as)
     constructor
     · exact det_automata_fin_run_exists al.length as
-    · simp [automata_congr_run, as]
+    · simp [automaton_congr_run, as]
 
 end Congruences
-
-section FiniteIndexCongruences
-
-variable {A : Type} {c : Congruence A}
-
-theorem fin_index_congr_regular [Inhabited A]
-    (h : Finite (Quotient c.eq)) (s : Quotient c.eq) : RegLang (Quotient.mk c.eq ⁻¹' {s}) := by
-  use (FromDetAutomaton (AutomataCongr c)), {s}
-  constructor
-  · exact h
-  · symm ; exact accepted_lang_congr s
-
-end FiniteIndexCongruences
