AutomataTheory.lean
@@ -1,5 +1,6 @@
 import AutomataTheory.AutomataBasic
 import AutomataTheory.AutomataConcat
+import AutomataTheory.AutomataCongr
 import AutomataTheory.AutomataDet
 import AutomataTheory.AutomataHist
 import AutomataTheory.AutomataLoop
@@ -7,7 +8,6 @@ import AutomataTheory.AutomataOI2
 import AutomataTheory.AutomataPSet
 import AutomataTheory.AutomataProd
 import AutomataTheory.AutomataSum
-import AutomataTheory.Congruences
 import AutomataTheory.Languages
 import AutomataTheory.OmegaRegLang
 import AutomataTheory.RegLang
